SciLean/Data/DataArray.lean
@@ -1,3 +1,4 @@
 import SciLean.Data.DataArray.PlainDataType
 import SciLean.Data.DataArray.DataArray
 import SciLean.Data.DataArray.VecN
+import SciLean.Data.DataArray.Operations
