SciLean/Data/DataArray/Operations.lean
@@ -1,0 +1,39 @@
+import SciLean.Data.DataArray.DataArray
+
+namespace SciLean.DataArrayN
+
+abbrev mapMono [IndexType I] [PlainDataType X]
+    (x : DataArrayN X I) (f : X → X) :=
+  ArrayType.mapMono f x
+
+abbrev mapIdxMono [IndexType I] [PlainDataType X]
+    (x : DataArrayN X I) (f : I → X → X) :=
+  ArrayType.mapIdxMono f x
+
+
+abbrev fold [IndexType I] [PlainDataType X]
+    (x : DataArrayN X I) (f : Y → X → Y) (init : Y):=
+  LeanColls.Fold.fold x f init
+
+abbrev foldIdx [IndexType I] [PlainDataType X]
+    (x : DataArrayN X I) (f : I → Y → X → Y) (init : Y) :=
+  LeanColls.Fold.fold (LeanColls.Indexed.WithIdx.mk x) (fun y (i,x) => f i y x) init
+
+abbrev reduceD [IndexType I] [PlainDataType X]
+    (x : DataArrayN X I) (f : X → X → X) (default : X):=
+  IndexType.reduceD (fun i => x[i]) f default
+
+abbrev reduce [IndexType I] [PlainDataType X] [Inhabited X]
+    (x : DataArrayN X I) (f : X → X → X) :=
+  IndexType.reduce (fun i => x[i]) f
+
+
+
+
+abbrev max [IndexType I] [PlainDataType X] [Max X] [Inhabited X]
+    (x : DataArrayN X I) : X :=
+  IndexType.reduce (fun i : I => x[i]) (Max.max · ·)
+
+abbrev min [IndexType I] [PlainDataType X] [Min X] [Inhabited X]
+    (x : DataArrayN X I) : X :=
+  IndexType.reduce (fun i : I => x[i]) (Min.min · ·)
