SciLean/Tactic/DeduceBy.lean
@@ -1,0 +1,100 @@
+import Lean
+import Qq
+
+import Mathlib.Tactic.NormNum.Basic
+import Mathlib.Tactic.NormNum.Result
+import Mathlib.Tactic.FieldSimp
+import Mathlib.Data.UInt
+import Mathlib.Tactic.Ring
+
+import SciLean.Util.RewriteBy
+
+namespace SciLean
+
+syntax (name:=deduceBy) "deduce_by " conv : tactic
+
+namespace DeduceBy
+open Qq Lean Meta
+
+/--
+Assuming that `a` has mvar `m` and `b` is an expression.
+
+Return mvar `m` and value `x` for it such that `a=b` is likely to hold.
+
+Examples:
+- `a = 4 * ?m + 2`, `b = 2*n` => `(?m, (2*n-2)/4)`
+-/
+partial def invertNat (a b : Q(Nat)) : MetaM (Q(Nat) × Q(Nat)) := do
+  if a.isMVar then
+    return (a,b)
+  else
+    match a with
+    | ~q($x * $y) =>
+      if x.hasMVar
+      then invertNat x q($b / $y)
+      else invertNat y q($b / $x)
+    | ~q($x / $y) =>
+      if x.hasMVar
+      then invertNat x q($b * $y)
+      else invertNat y q($x / $b)
+    | ~q($x + $y) =>
+      if x.hasMVar
+      then invertNat x q($b - $y)
+      else invertNat y q($b - $x)
+    | ~q($x - $y) =>
+      if x.hasMVar
+      then invertNat x q($b + $y)
+      else invertNat y q($x - $b)
+    | _ =>
+      throwError s!"`decuce_by` does not support Nat operation {← ppExpr a}"
+
+
+open Lean Meta Elab Tactic Qq
+@[tactic deduceBy]
+partial def deduceByTactic : Tactic
+| `(tactic| deduce_by $t:conv) => do
+
+  let goal ← getMainGoal
+  let .some (_,lhs,rhs) := Expr.eq? (← goal.getType) | throwError "expected `?m = e`, got {← ppExpr (← goal.getType)}"
+
+  -- if ¬lhs.isMVar then
+  --   throwError "lhs is not mvar"
+
+  -- now we assume that a is mvar and b is and expression we want to simplify
+  let (goal,a,b) ←
+    if lhs.hasMVar then
+      pure (goal,lhs,rhs)
+    else
+      let goal' ← mkFreshExprMVar (← mkEq rhs lhs)
+      goal.assign (← mkEqSymm goal')
+      pure (goal'.mvarId!,rhs,lhs)
+
+  let A ← inferType a
+  if A == q(Nat) then
+    let (m,x) ← invertNat a b
+    let (x', _) ← elabConvRewrite x #[] t
+    m.mvarId!.assign x'
+    let subgoals ← evalTacticAt (← `(tactic| (conv => (conv => lhs; $t); (conv => rhs; $t)); try field_simp)) goal
+    if subgoals.length ≠ 0 then
+      throwError "`decide_by` failed to show {← ppExpr (← goal.getType)}"
+
+  else
+    let (b',prf) ← elabConvRewrite b #[] t
+    a.mvarId!.assign b'
+    goal.assign prf
+| _ => throwUnsupportedSyntax
+
+
+-- def foo {n : Nat} {m : Nat} (i : Fin n) (h : 2 * m = n := by deduce_by ring_nf) : Fin m := ⟨i/2, sorry⟩
+
+-- def bar {n : Nat} (i : Fin n) : Fin (n/2) := ⟨i/2, sorry⟩
+
+-- variable (n : Nat)
+
+-- #check foo (8 : Fin 10)
+-- #eval foo (8 : Fin 10)
+
+-- #check bar (8 : Fin 10)
+
+-- variable (i : Fin (2*n))
+-- #eval foo i
